change BufferStack and BufferSeq, broken refinement proofs

Splinter/Betree/Buffer.i.dfy
@@ -10,6 +10,21 @@ module BufferMod
   import opened ValueMessage
   // import opened MessageMod
 
+  // TotalMapMod provides something like these, but it depends on module
+  // refinement that's hairy and has problems in use (rank_is_less_than doesn't
+  // make it through the module refinement, so we can't prove decreases).
+  predicate AnyKey(key: Key) { true }
+
+  predicate Total(keys: iset<Key>) {
+    forall k | AnyKey(k) :: k in keys
+  }
+
+  function AllKeys() : (out: iset<Key>)
+    ensures Total(out)
+  {
+    iset k | AnyKey(k)
+  }
+
   datatype Buffer = Buffer(mapp: map<Key, Message>)
   {
     function Query(key: Key) : Message
