Splinter/Betree/OffsetMap.i.dfy
@@ -9,20 +9,6 @@ module OffsetMapMod {
   import opened KeyType
   import opened BufferMod
 
-
-  // TotalMapMod provides something like these, but it depends on module
-  // refinement that's hairy and has problems in use (rank_is_less_than doesn't
-  // make it through the module refinement, so we can't prove decreases).
-  predicate AnyKey(key: Key) { true }
-  predicate Total(keys: iset<Key>) {
-    forall k | AnyKey(k) :: k in keys
-  }
-  function AllKeys() : (out: iset<Key>)
-    ensures Total(out)
-  {
-    iset k | AnyKey(k)
-  }
-
   datatype OffsetMap = OffsetMap(offsets: imap<Key, nat>)
   {
     predicate WF() {
